iris/UserMem.v
@@ -98,10 +98,8 @@ Proof.
   rewrite pma_ok_aligned_splittable pma_ok_aligned_granule.
   rewrite (execR_liftR_seq _ _ _ _ _ (exec_split_misaligned_unsplit addr 2 0 s)). cbn beta.
   rewrite misaligned_order_1. cbn zeta.
-  rewrite (execR_liftR_seq _ _ _ _ _
-             (_ : exec (read_kind_of_flags _ _ false) s = Some (rv64d_types.Read_plain, s))).
-  2:{ unfold read_kind_of_flags. apply exec_returnM. }
-  cbn beta.
+  (* the read kind: an instruction fetch takes [rk_select]'s [Read_ifetch] arm *)
+  cbn match. rewrite mbind_returnR. cbn beta.
   match goal with |- context[Defs.bind (Defs.untilMT ?vs ?m ?c ?b) _] =>
     assert (Hu : execR (Defs.untilMT vs m c b) s = Some (inr (w, true, 0), s)) end.
   { eapply execR_untilMT_1; [ reflexivity | | apply execR_returnR_fwd ].
@@ -121,7 +119,7 @@ Proof.
       |- context[Defs.bind (Defs.bind (Defs.liftR (read_ram ?rk ?pa ?wd ?mt)) ?k1) _] =>
       assert (Hrd : execR (Defs.bind (Defs.liftR (read_ram rk pa wd mt)) k1) s
                     = Some (inr w, s)) end.
-    { rewrite (execR_liftR_seq _ _ _ _ _ (exec_read_ram_plain_2 addr w s Hdev Hbytes)).
+    { rewrite (execR_liftR_seq _ _ _ _ _ (exec_read_ram_ifetch_2 addr w s Hdev Hbytes)).
       cbn beta match. apply execR_returnR_fwd. }
     rewrite (execR_bind_Some _ _ _ _ _ Hrd). cbn beta zeta.
     rewrite autocast_id. rewrite usvd_zeros_full_16.
@@ -204,10 +202,8 @@ Proof.
   rewrite pma_ok_aligned_splittable pma_ok_aligned_granule.
   rewrite (execR_liftR_seq _ _ _ _ _ (exec_split_misaligned_unsplit addr 4 0 s)). cbn beta.
   rewrite misaligned_order_1. cbn zeta.
-  rewrite (execR_liftR_seq _ _ _ _ _
-             (_ : exec (read_kind_of_flags _ _ false) s = Some (rv64d_types.Read_plain, s))).
-  2:{ unfold read_kind_of_flags. apply exec_returnM. }
-  cbn beta.
+  (* the read kind: an instruction fetch takes [rk_select]'s [Read_ifetch] arm *)
+  cbn match. rewrite mbind_returnR. cbn beta.
   match goal with |- context[Defs.bind (Defs.untilMT ?vs ?m ?c ?b) _] =>
     assert (Hu : execR (Defs.untilMT vs m c b) s = Some (inr (w, true, 0), s)) end.
   { eapply execR_untilMT_1; [ reflexivity | | apply execR_returnR_fwd ].
@@ -227,7 +223,7 @@ Proof.
       |- context[Defs.bind (Defs.bind (Defs.liftR (read_ram ?rk ?pa ?wd ?mt)) ?k1) _] =>
       assert (Hrd : execR (Defs.bind (Defs.liftR (read_ram rk pa wd mt)) k1) s
                     = Some (inr w, s)) end.
-    { rewrite (execR_liftR_seq _ _ _ _ _ (exec_read_ram_plain_4 addr w s Hdev Hbytes)).
+    { rewrite (execR_liftR_seq _ _ _ _ _ (exec_read_ram_ifetch_4 addr w s Hdev Hbytes)).
       cbn beta match. apply execR_returnR_fwd. }
     rewrite (execR_bind_Some _ _ _ _ _ Hrd). cbn beta zeta.
     rewrite autocast_id. rewrite usvd_zeros_full_32.
