iris/WpSmodePtMem.v
@@ -89,7 +89,7 @@ Local Lemma exec_checked_mem_read_ram_load_4_S (pbmt : page_based_mem_type) (add
     assert (Hrkf : exec (read_kind_of_flags false false false) s
                    = Some (rv64d_types.Read_plain, s))
       by (unfold read_kind_of_flags; apply exec_returnM).
-    rewrite (execR_liftR_seq _ _ _ _ _ Hrkf). cbn beta.
+    cbn match. rewrite (execR_liftR_seq _ _ _ _ _ Hrkf). cbn beta.
     match goal with |- context[Defs.bind (Defs.untilMT ?vs ?m0 ?c ?bb) _] =>
       assert (Hu : execR (Defs.untilMT vs m0 c bb) s = Some (inr (w, true, 0), s)) end.
     { eapply execR_untilMT_1; [ reflexivity | | apply execR_returnR_fwd ].
